ML -> Isar

src/HOL/Lex/RegSet.thy
@@ -6,16 +6,32 @@
 Regular sets
 *)
 
-RegSet = Main +
+theory RegSet = Main:
 
 constdefs
- conc :: 'a list set => 'a list set => 'a list set
+ conc :: "'a list set => 'a list set => 'a list set"
 "conc A B == {xs@ys | xs ys. xs:A & ys:B}"
 
-consts star :: 'a list set => 'a list set
+consts star :: "'a list set => 'a list set"
 inductive "star A"
-intrs
-  NilI   "[] : star A"
-  ConsI  "[| a:A; as : star A |] ==> a@as : star A"
+intros
+  NilI[iff]:   "[] : star A"
+  ConsI[intro,simp]:  "[| a:A; as : star A |] ==> a@as : star A"
+
+lemma concat_in_star: "!xs: set xss. xs:S ==> concat xss : star S"
+by (induct "xss") simp_all
+
+lemma in_star:
+ "w : star U = (? us. (!u : set(us). u : U) & (w = concat us))"
+apply (rule iffI)
+ apply (erule star.induct)
+  apply (rule_tac x = "[]" in exI)
+  apply simp
+ apply clarify
+ apply (rule_tac x = "a#us" in exI)
+ apply simp
+apply clarify
+apply (simp add: concat_in_star)
+done
 
 end
